Kura/Connectivity/Tree.lean
@@ -21,9 +21,48 @@ lemma SubgraphOf.acyclic {G : Graph V E} {H : Graph W F} (hHG : H ⊆ᴳ G) : G.
   exact h.trans hHG
 
 lemma endAt_not_conn {G : Graph V E} [Undirected G] (hGacyc : G.acyclic) (e : E) :
-    ¬ G.conn (G.v1 e) (G.v2 e) := by
-  rintro hconn
-  
+    ¬ (G{{e}ᶜ}ᴳ).conn (G.v1 e) (G.v2 e) := by
+  contrapose! hGacyc
+  obtain ⟨n, S, hs, ht⟩ := hGacyc.PathSubgr
+  simp only [acyclic, not_forall, not_isEmpty_iff]
+  use n.succPNat
+  refine ⟨(TourGraph_Isom_PathGraph_addUndirEdge n).toSubgraphOf.trans ?_⟩
+  refine ⟨⟨S.fᵥ, ?_,?_⟩,?_,?_⟩
+  · intro e'
+    match e' with
+    | Sum.inl e => exact S.fₑ e |>.val
+    | Sum.inr () => exact e
+  · intro e'
+    match e' with
+    | Sum.inl e' =>
+      simp only [addUndirEdge_inc_inl]
+      rw [← S.inc e', Es_inc]
+    | Sum.inr () =>
+      simp only
+      rw [addUndirEdge_inc_inr, map_undir, inc_eq_undir_v12]
+      congr
+      exact hs.symm
+      convert ht.symm
+      exact (Fin.natCast_eq_last n).symm
+  · rintro e₁ e₂ h
+    simp at h
+    exact S.fᵥinj h
+  · rintro e₁ e₂ h
+    match e₁, e₂ with
+    | Sum.inl e₁, Sum.inl e₂ =>
+      simp only [S.inc, addUndirEdge_inc_inl] at h
+      congr
+      exact S.fₑinj <| Subtype.val_injective h
+    | Sum.inr (), Sum.inr () => rfl
+    | Sum.inl e', Sum.inr () =>
+      simp only at h
+      have := h ▸ (S.fₑ e').prop
+      simp only [Set.mem_compl_iff, Set.mem_singleton_iff, not_true_eq_false] at this
+    | Sum.inr (), Sum.inl e' =>
+      simp only at h
+      have := h.symm ▸ (S.fₑ e').prop
+      simp only [Set.mem_compl_iff, Set.mem_singleton_iff, not_true_eq_false] at this
+
 
 theorem n_eq_m_add_c_of_acyclic [Fintype V] [Fintype E] {G : Graph V E} [Undirected G]
     (hG : G.acyclic) : Fintype.card V = Fintype.card E + NumberOfComponents G := by
@@ -45,10 +84,45 @@ theorem n_eq_m_add_c_of_acyclic [Fintype V] [Fintype E] {G : Graph V E} [Undirec
     specialize ih (G := G{{e}ᶜ}ᴳ) (hG'Subgr.acyclic hG) ?_
     · rw [Fintype.card_compl_set, hm]
       simp only [Fintype.card_ofSubsingleton, add_tsub_cancel_right]
-    rw [ih]
+    rw [ih]; clear hm ih
     suffices (G.Es {e}ᶜ).NumberOfComponents = 1 + G.NumberOfComponents by rw [this]; omega
+    apply le_antisymm
+    · unfold NumberOfComponents
+      rw [add_comm, ← @Fintype.card_option]
+      let f : Quotient (G.Es {e}ᶜ).connSetoid → Option (Quotient G.connSetoid) :=
+        fun v ↦ by
+          by_cases h : v = ⟦G.v2 e⟧
+          · exact none
+          · exact some (Quotient.idmap (G.connSetoid_Es_le_connSetoid _) v)
+      convert Fintype.card_le_of_injective f ?_
+      rintro v w h
+      unfold f at h
+      by_cases hv : v = ⟦G.v2 e⟧ <;> by_cases hw : w = ⟦G.v2 e⟧ <;> simp_all [dite_eq_ite,
+        ite_false, Option.some.injEq]
+      induction' v using Quotient.ind with v
+      induction' w using Quotient.ind with w
+      simp_all only [connSetoid, Quotient.eq, Quotient.idmap, Quotient.map'_mk'', id_eq]
+      obtain ⟨n, S, hs, ht⟩ := h.PathSubgr
+      by_cases hv2 : ∃ n, S.fᵥ n = G.v2 e
+      · exfalso
+        -- have := PathGraph_SubgraphOf_Pathgraph
+        sorry
 
-    sorry
+      · simp only [not_exists] at hv2
+        obtain a := S.Es (PathGraph n) {e}ᶜ sorry
+        
+        sorry
+    · suffices G.NumberOfComponents < (G.Es {e}ᶜ).NumberOfComponents by omega
+      unfold NumberOfComponents
+      convert Quotient.card_quotient_lt_card_quotient_of_gt (?_ : _ < G.connSetoid)
+      rw [lt_iff_le_and_ne]
+      refine ⟨G.connSetoid_Es_le_connSetoid _, ?_⟩
+      have h := endAt_not_conn hG e
+      contrapose! h
+      have : (G.Es {e}ᶜ).connSetoid (G.v1 e) (G.v2 e) ↔ G.connSetoid (G.v1 e) (G.v2 e) := by rw [h]
+      simp only [connSetoid] at this
+      rw [this]; clear this h
+      apply conn.ofAdj <| adj_v12 G e
 
 structure Forest (V E : Type*) [DecidableEq V] extends Graph V E where
   no_cycle : IsEmpty toGraph.Cycle
